New approach to Stackingproof
There are two aspects of the Stacking pass which conspire
to make things difficult. One one hand, the stacking simulation
relation is fairly complex to begin with. On the other hand,
for various reasons splitting the simulation convention into
a structural component and a CKLR component is more difficult
than with other translation passes.

To make this easier to deal with, I separate concerns by
verifying Stacking against a monolithic simulation convention
[cc_stacking], then prove a correspondance between that
simulation convention and the ones we use for commutation
properties.

backend/Mach.v
@@ -490,62 +490,7 @@ Definition semantics (rao: function -> code -> ptrofs -> Prop) (p: program) :=
 
 (** * Simulation conventions *)
 
-(** ** Calling convention from [li_locset] *)
-
-(** A key aspect concerns the encoding of arguments in the memory.
-  Arguments may be found in assembly stack frames, but the source
-  program must not have access to them. So we assert that the source
-  memory is equal to the target memory, but in the source the
-  permissions for the stack's arguments area has been removed. *)
-
-Import Stacklayout.
-
-Fixpoint loc_footprints (sb: block) (sofs: ptrofs) (l: list loc) :=
-  match l with
-    | S Outgoing ofs ty :: l' =>
-      let lo := Ptrofs.unsigned (Ptrofs.add (Ptrofs.repr (fe_ofs_arg + 4 * ofs)) sofs) in
-      (sb, lo, lo + size_chunk (chunk_of_type ty)) :: loc_footprints sb sofs l'
-    | _ :: l' => loc_footprints sb sofs l'
-    | nil => nil
-  end.
-
-Definition free_args (sg: signature) (m: mem) (sp: val) :=
-  match sp with
-    | Vptr sb sofs =>
-      Mem.free_list m (loc_footprints sb sofs (regs_of_rpairs (loc_arguments sg)))
-    | _ =>
-      None
-  end.
-
-Definition agree_args (sg: signature) (m: mem) (sp: val) (ls: Locmap.t) :=
-  forall ofs ty,
-    let l := S Outgoing ofs ty in
-    In l (regs_of_rpairs (loc_arguments sg)) ->
-    load_stack m sp ty (Ptrofs.repr (fe_ofs_arg + 4 * ofs)) = Some (ls l).
-
-Inductive cc_locset_mach_mq sg rs: locset_query -> mach_query -> Prop :=
-  cc_locset_mach_mq_intro vf ls sp ra m m':
-    (*Mem.valid_block m sp -> *)
-    Val.has_type ra Tptr ->
-    free_args sg m sp = Some m' ->
-    (forall r, ls (R r) = rs r) ->
-    agree_args sg m sp ls ->
-    cc_locset_mach_mq sg rs (lq vf sg ls m') (mq vf sp ra rs m).
-
-Inductive cc_locset_mach_mr sg rs: locset_reply -> mach_reply -> Prop :=
-  cc_locset_mach_mr_intro ls' rs' m':
-    (forall r, is_callee_save r = true -> rs' r = rs r) ->
-    (forall r, In r (regs_of_rpair (loc_result sg)) -> rs' r = ls' (R r)) ->
-    cc_locset_mach_mr sg rs (lr ls' m') (mr rs' m').
-
-Program Definition cc_locset_mach: callconv li_locset li_mach :=
-  {|
-    match_senv _ := eq;
-    match_query '(sg, rs) := cc_locset_mach_mq sg rs;
-    match_reply '(sg, rs) := cc_locset_mach_mr sg rs;
-  |}.
-
-(** ** CKLR simulation conventions *)
+(** ** CKLR simulation convention *)
 
 Inductive cc_mach_mq R w: mach_query -> mach_query -> Prop :=
   cc_mach_mq_intro vf1 vf2 sp1 sp2 ra1 ra2 rs1 rs2 m1 m2:
@@ -577,32 +522,147 @@ Next Obligation.
   eapply match_stbls_proj in H. erewrite <- Genv.valid_for_match; eauto.
 Qed.
 
-(** ** Properties *)
+(** ** Calling convention from [li_locset] *)
 
-Lemma nextblock_free_args sg m sp m':
-  free_args sg m sp = Some m' ->
-  Mem.nextblock m' = Mem.nextblock m.
+(** A key aspect concerns the encoding of arguments in the memory.
+  Arguments may be found in assembly stack frames, but the source
+  program must not have access to them. So we assert that the source
+  memory is equal to the target memory, but in the source the
+  permissions for the stack's arguments area has been removed. *)
+
+Require Import Stacklayout.
+
+(** One complication occurs for compatibility with CKLRs. When the
+  arguments region is non-empty, success of the source-level
+  [Mem.free] ensures that the corresponding pointer [sp + fe_ofs_arg]
+  is valid, hence injects into the target-level one. But if the
+  argument region is empty, we do not have a similar guarantee.
+  For example, for the initial invocation of [main()] with empty
+  arguments, the stack pointer is not even of the form [Vptr b ofs]
+  but is instead a zero integer.
+
+  In addition to addressing this, we must make sure that accesses to
+  the arguments region formulated in terms of concrete binary pointers
+  correspond to the range freed in terms of abstract integer addresses.
+
+  This is handled by the following construction. *)
+
+Require Import Separation.
+Local Open Scope sep_scope.
+
+Definition offset_sarg sofs ofs :=
+  Ptrofs.unsigned sofs + (fe_ofs_arg + 4 * ofs).
+
+Definition offset_fits sofs ofs :=
+  ofs >= 0 /\ offset_sarg sofs ofs <= Ptrofs.max_unsigned.
+
+Lemma access_fits sofs ofs:
+  offset_fits sofs ofs ->
+  offset_sarg sofs ofs =
+  Ptrofs.unsigned (Ptrofs.add sofs (Ptrofs.repr (fe_ofs_arg + 4 * ofs))).
 Proof.
-  destruct sp; try discriminate. cbn. revert m.
-  induction (loc_footprints b i (regs_of_rpairs (loc_arguments sg))); cbn.
-  - congruence.
-  - intros. destruct a as [[? ?] ?], Mem.free eqn:Hm'; try congruence.
-    erewrite <- (Mem.nextblock_free m _ _ _ m0); eauto.
+  unfold offset_fits, offset_sarg.
+  intros [OPOS FITS].
+  assert (fe_ofs_arg >= 0) by (unfold fe_ofs_arg; xomega).
+  pose proof (Ptrofs.unsigned_range_2 sofs).
+  rewrite !Ptrofs.add_unsigned.
+  rewrite (Ptrofs.unsigned_repr (fe_ofs_arg + _)) by xomega.
+  rewrite (Ptrofs.unsigned_repr (_ + _)) by xomega.
+  reflexivity.
 Qed.
 
-(** The following construction is needed both for the commutation
-  property associated with [cc_locset_mach] and [cc_mach] and in the
-  simulation proof for external calls in [Stacking]. It is used to
-  formulate an [li_locset] view of an [li_mach] query. *)
+Inductive loc_init_args sb sofs sz : block -> Z -> Prop :=
+  loc_init_args_intro ofs:
+    offset_sarg sofs 0 <= ofs < offset_sarg sofs sz ->
+    loc_init_args sb sofs sz sb ofs.
 
-Definition make_locset (rs: regset) (m: mem) (sp: val) (l: loc) : val :=
-  match l with
-    | R r => rs r
-    | S Outgoing ofs ty =>
-      let v := load_stack m sp ty (Ptrofs.repr (fe_ofs_arg + 4 * ofs)) in
-      Val.maketotal v
-    | _ => Vundef
-  end.
+Program Definition contains_init_args sg j ls m0 sb sofs : massert :=
+  let sz := size_arguments sg in
+  {|
+    m_pred m :=
+      Mem.range_perm m sb (offset_sarg sofs 0) (offset_sarg sofs sz) Cur Freeable /\
+      Mem.unchanged_on (loc_init_args sb sofs sz) m0 m /\
+      (forall ofs, 0 <= ofs < sz -> offset_fits sofs ofs) /\
+      (forall ofs ty,
+        In (S Outgoing ofs ty) (regs_of_rpairs (loc_arguments sg)) ->
+        exists v,
+          Mem.load (chunk_of_type ty) m sb (offset_sarg sofs ofs) = Some v /\
+          Val.inject j (ls (S Outgoing ofs ty)) v);
+    m_footprint := loc_init_args sb sofs sz;
+  |}.
+Next Obligation.
+  repeat apply conj.
+  - intros ofs Hofs. erewrite <- Mem.unchanged_on_perm; eauto.
+    + constructor; auto.
+    + eapply Mem.perm_valid_block; eauto.
+  - eapply Mem.unchanged_on_trans; eauto.
+  - auto.
+  - intros ofs ty REG. edestruct H3 as (? & ? & ?); eauto.
+    pose proof (loc_arguments_bounded _ _ _ REG).
+    pose proof (loc_arguments_acceptable_2 _ _ REG) as [? _].
+    eexists; split; eauto. eapply Mem.load_unchanged_on; eauto.
+    intros. constructor. unfold offset_sarg in *.
+    destruct ty; cbn [typesize size_chunk chunk_of_type] in *; xomega.
+Qed.
+Next Obligation.
+  destruct H0 as [ofs Hofs].
+  eapply Mem.perm_valid_block; eauto.
+Qed.
+
+Record cc_stacking_world {R} :=
+  stkw {
+    stk_w :> world R;
+    stk_sg : signature;
+    stk_ls1 : Locmap.t;
+    stk_sb2 : block;
+    stk_sofs2 : ptrofs;
+    stk_m2 : mem;
+  }.
+
+Arguments cc_stacking_world : clear implicits.
+
+Inductive cc_stacking_mq R: cc_stacking_world R -> _ -> _ -> Prop :=
+  | cc_stacking_mq_intro w vf1 vf2 sg ls1 m1 sb2 sofs2 ra2 rs2 m2:
+      vf1 <> Vundef -> Val.inject (mi R w) vf1 vf2 ->
+      (forall r, Val.inject (mi R w) (ls1 (Locations.R r)) (rs2 r)) ->
+      m2 |= contains_init_args sg (mi R w) ls1 m2 sb2 sofs2 ->
+      match_mem R w m1 m2 ->
+      (forall b ofs, loc_init_args sb2 sofs2 (size_arguments sg) b ofs ->
+                     loc_out_of_reach (mi R w) m1 b ofs) ->
+      (*ra2 <> Vundef ->*) Val.has_type ra2 Tptr ->
+      cc_stacking_mq R
+        (stkw R w sg ls1 sb2 sofs2 m2)
+        (lq vf1 sg ls1 m1)
+        (mq vf2 (Vptr sb2 sofs2) ra2 rs2 m2).
+
+Inductive cc_stacking_mr R: cc_stacking_world R -> _ -> _ -> Prop :=
+  | cc_stacking_mr_intro w w' sg ls1 ls1' m1' sb2 sofs2 m2 rs2' m2':
+    w ~> w' ->
+    (forall r,
+      In r (regs_of_rpair (loc_result sg)) ->
+      Val.inject (mi R w') (ls1' (Locations.R r)) (rs2' r)) ->
+    (forall r,
+      is_callee_save r = true ->
+      Val.inject (mi R w') (ls1 (Locations.R r)) (rs2' r)) ->
+    match_mem R w' m1' m2' ->
+    Mem.unchanged_on (loc_init_args sb2 sofs2 (size_arguments sg)) m2 m2' ->
+    cc_stacking_mr R
+      (stkw R w sg ls1 sb2 sofs2 m2)
+      (lr ls1' m1')
+      (mr rs2' m2').
+
+Program Definition cc_stacking R: callconv li_locset li_mach :=
+  {|
+    match_senv := (match_stbls R @@ [stk_w])%klr;
+    match_query := cc_stacking_mq R;
+    match_reply := cc_stacking_mr R;
+  |}.
+Next Obligation.
+  eapply (LanguageInterface.cc_c_obligation_1 R w se1 se2 H); eauto.
+Qed.
+Next Obligation.
+  eapply (LanguageInterface.cc_c_obligation_2 R w se1 se2 sk H); eauto.
+Qed.
 
 (** ** To relocate or remove *)
 
